monadproofs/proofs/prelude.v
@@ -1,0 +1,17 @@
+(* TODO: put most Imports in a prelude *)
+Require Export monad.proofs.misc.
+Require Export monad.proofs.evmopsem.
+Require Export monad.asts.exb.
+Require Export bluerock.auto.cpp.spec.
+Require Export monad.proofs.libspecs.
+Export cQp_compat.
+Open Scope lens_scope.
+Open Scope Z_scope.
+Open Scope N_scope.
+(*
+Require Import EVMOpSem.evmfull. *)
+Export cancelable_invariants.
+Require Export monad.proofs.exec_specs.
+Export linearity.
+Export libspecs.
+
